eq compat lemmas, Kuratowski's pair, rank

theories/Data/Aczel.v
@@ -68,6 +68,12 @@ Definition childnodes (x : Tree) : forall c : children x, Tree :=
   | mkNode _ ts => ts
   end.
 
+Lemma Tree_eta x
+  : mkNode (children x) (childnodes x) = x.
+Proof.
+  destruct x as [csx tsx]; reflexivity.
+Defined.
+
 Definition member (x : Tree) (y : Tree) : Prop :=
   exists c : children y, x == childnodes y c.
 
@@ -128,6 +134,8 @@ Defined.
 #[global] Hint Resolve eqTree_Reflexive eqTree_Symmetric eqTree_Transitive : aczel_hints.
 
 #[local] Hint Resolve Equivalence_Reflexive Equivalence_Symmetric Equivalence_Transitive : core.
+
+#[local] Hint Resolve eqProp_refl eqProp_sym eqProp_trans leProp_refl leProp_trans leProp_antisymmetry eqProp_implies_leProp : core.
 
 #[global] Hint Unfold children childnodes member : aczel_hints.
 
@@ -239,6 +247,14 @@ Proof.
   - intros [[c EQ] H_P]. exists c. done.
 Qed.
 
+#[global]
+Instance filter_eqPropCompatible1 P
+  (COMPAT : isCompatibleWith_eqProp P)
+  : eqPropCompatible1 (filter P).
+Proof.
+  now ii; eapply eqTree_intro; ii; rewrite filter_good in *; eauto with *; [rewrite <- x_EQ | rewrite -> x_EQ].
+Qed.
+
 Definition power (x : Tree) : Tree :=
   mkNode (children x -> Prop) (filterc x).
 
@@ -246,6 +262,13 @@ Theorem power_spec x
   : forall z, z \in power x <-> z \subseteq x.
 Proof.
   intros z. rewrite subset_filterc. unfold power. eauto with *.
+Qed.
+
+#[global]
+Instance power_eqPropCompatible1
+  : eqPropCompatible1 power.
+Proof.
+  ii; eapply eqTree_intro; ii; rewrite power_spec in *; ii; [rewrite <- x_EQ | rewrite -> x_EQ]; eauto.
 Qed.
 
 Definition indexed_union (I : Type@{Set_u}) (x_i : I -> Tree) : Tree :=
@@ -259,15 +282,30 @@ Proof.
   - intros [i [c EQ]]; simpl in *; exists (@existT _ _ i c); eauto with *.
 Qed.
 
-Definition bigcup (x : Tree) : Tree :=
+#[global]
+Instance indexed_union_eqPropCompatible1 I
+  : eqPropCompatible1 (indexed_union I).
+Proof.
+  ii. change (forall i : I, x1 i == x2 i) in x_EQ.
+  eapply eqTree_intro; ii; rewrite indexed_union_spec in *; des; exists i; [rewrite <- x_EQ | rewrite -> x_EQ]; eauto with *.
+Qed.
+
+Definition unions (x : Tree) : Tree :=
   indexed_union (children x) (childnodes x).
 
-Theorem bigcup_spec x
-  : forall z, z \in bigcup x <-> exists y, z \in y /\ y \in x.
+Theorem unions_spec x
+  : forall z, z \in unions x <-> exists y, z \in y /\ y \in x.
 Proof.
-  intros z. unfold bigcup. rewrite indexed_union_spec. split.
+  intros z. unfold unions. rewrite indexed_union_spec. split.
   - intros [i [c EQ]]; simpl in *; exists (childnodes x i); split; eauto with *.
   - intros [y [IN [c EQ]]]; simpl in *. exists c. rewrite <- EQ. exact IN.
+Qed.
+
+#[global]
+Instance unions_eqPropCompatible1
+  : eqPropCompatible1 unions.
+Proof.
+  ii; eapply eqTree_intro; ii; rewrite unions_spec in *; des; exists y; [rewrite <- x_EQ | rewrite -> x_EQ]; done.
 Qed.
 
 Definition empty : Tree :=
@@ -292,25 +330,223 @@ Proof.
   - intros [EQ | EQ]; [exists true | exists false]; eauto with *.
 Qed.
 
+#[global]
+Instance upair_eqPropCompatible2
+  : eqPropCompatible2 upair.
+Proof.
+  ii; eapply eqTree_intro; ii; rewrite upair_spec in *; [rewrite <- x_EQ, <- y_EQ | rewrite -> x_EQ, -> y_EQ]; eauto with *.
+Qed.
+
+#[global]
+Instance upair_comm
+  : isCommutative upair.
+Proof.
+  ii. eapply eqTree_intro; ii; rewrite upair_spec in *; done.
+Qed.
+
 Definition union (x1 : Tree) (x2 : Tree) : Tree :=
-  bigcup (upair x1 x2).
+  unions (upair x1 x2).
 
 Theorem union_spec x1 x2
   : forall z, z \in union x1 x2 <-> z \in x1 \/ z \in x2.
 Proof.
-  intros z. unfold union. rewrite bigcup_spec. split.
+  intros z. unfold union. rewrite unions_spec. split.
   - intros [y [IN IN']]; rewrite upair_spec in IN'.
     destruct IN' as [EQ | EQ]; rewrite EQ in IN; eauto.
   - intros [IN | IN]; [exists x1 | exists x2]; rewrite upair_spec; eauto with *.
 Qed.
 
-Definition singleton (x : Tree) : Tree :=
+#[global]
+Instance union_eqPropCompatible2
+  : eqPropCompatible2 union.
+Proof.
+  ii; eapply eqTree_intro; ii; rewrite union_spec in *; [rewrite <- x_EQ, <- y_EQ | rewrite -> x_EQ, -> y_EQ]; eauto with *.
+Qed.
+
+Definition singlton (x : Tree) : Tree :=
   upair x x.
 
-Theorem singleton_spec x
-  : forall z, z \in singleton x <-> z == x.
+Theorem singlton_spec x
+  : forall z, z \in singlton x <-> z == x.
 Proof.
-  intros z. unfold singleton. rewrite upair_spec. done.
+  intros z. unfold singlton. rewrite upair_spec. done.
+Qed.
+
+Corollary singlton_inj x y
+  (EQ : singlton x == singlton y)
+  : x == y.
+Proof.
+  assert (IN : x \in singlton x) by now rewrite singlton_spec.
+  rewrite EQ in IN. rewrite singlton_spec in IN. done.
+Qed.
+
+#[global]
+Instance singlton_eqPropCompatible1
+  : eqPropCompatible1 singlton.
+Proof.
+  ii. eapply eqTree_intro; ii.
+  - rewrite singlton_spec in *. rewrite <- x_EQ. exact H.
+  - rewrite singlton_spec in *. rewrite -> x_EQ. exact H.
+Qed.
+
+Lemma upair_eq_upair_implies x1 y1 x2 y2
+  (EQ : upair x1 y1 == upair x2 y2)
+  : (x1 == x2 /\ y1 == y2) \/ (x1 == y2 /\ x2 == y1).
+Proof.
+  assert (H_in : x1 \in upair x1 y1).
+  { rewrite upair_spec. now left. }
+  rewrite EQ in H_in. rewrite upair_spec in H_in.
+  destruct H_in as [H_EQ | H_EQ].
+  - left. split; trivial. rewrite H_EQ in EQ.
+    assert (IN : y1 \in upair x2 y1).
+    { rewrite upair_spec. now right. }
+    rewrite -> EQ in IN. rewrite upair_spec in IN.
+    destruct IN as [H_EQ' | H_EQ'].
+    + rewrite -> H_EQ'. symmetry. rewrite <- singlton_spec.
+      unfold singlton. rewrite -> H_EQ' in EQ. rewrite -> EQ.
+      rewrite upair_spec. now right.
+    + eauto with *.
+  - right. split; trivial. rewrite H_EQ in EQ.
+    assert (IN : x2 \in upair x2 y2).
+    { rewrite upair_spec. now left. }
+    rewrite <- EQ in IN. rewrite upair_spec in IN.
+    destruct IN as [H_EQ' | H_EQ'].
+    + rewrite -> H_EQ'. symmetry. rewrite <- singlton_spec.
+      unfold singlton. rewrite -> H_EQ' in EQ. rewrite <- EQ.
+      rewrite upair_spec. now right.
+    + eauto with *.
+Qed.
+
+Lemma singleton_eq_upair_implies x y z
+  (EQ : singlton x == upair y z)
+  : x == y /\ y == z.
+Proof.
+  revert x y z EQ. enough (WTS : forall x, forall y, forall z, singlton x == upair y z -> x == y).
+  { ii. enough (ENOUGH : x == y).
+    - split; trivial. rewrite comm in EQ. apply WTS in EQ. rewrite EQ in ENOUGH. done.
+    - eapply WTS. exact EQ.
+  }
+  intros x y z EQ. unfold singlton in EQ. apply upair_eq_upair_implies in EQ. destruct EQ as [[EQ1 H_EQ] | [EQ1 H_EQ]]; done.
+Qed.
+
+Definition pair (x : Tree) (y : Tree) : Tree :=
+  upair (singlton x) (upair x y).
+
+Theorem pair_inv x1 x2 y1 y2
+  (EQ : pair x1 y1 == pair x2 y2)
+  : x1 == x2 /\ y1 == y2.
+Proof.
+  unfold pair in EQ. apply upair_eq_upair_implies in EQ. destruct EQ as [[EQ1 H_EQ] | [EQ1 H_EQ]].
+  - apply singlton_inj in EQ1. split; trivial. apply upair_eq_upair_implies in H_EQ. destruct H_EQ as [[EQ2 EQ3] | [EQ2 EQ3]]; eauto with *.
+  - apply singleton_eq_upair_implies in H_EQ. apply singleton_eq_upair_implies in EQ1.
+    destruct EQ1 as [EQ1 EQ2], H_EQ as [EQ3 EQ4]. rewrite EQ4, EQ3, EQ1, EQ2. rewrite <- EQ4, <- EQ3, <- EQ2. now split.
+Qed.
+
+#[global]
+Instance pair_eqPropCompatible2
+  : eqPropCompatible2 pair.
+Proof.
+  ii. unfold pair. now rewrite x_EQ, y_EQ.
+Qed.
+
+Definition fst (t : Tree) : Tree :=
+  unions (filter (fun x => singlton x \in t) (unions t)).
+
+#[global]
+Instance fst_eqPropCompatible1
+  : eqPropCompatible1 fst.
+Proof.
+  ii. unfold fst. eapply eqTree_intro; ii; rewrite unions_spec in *.
+  - des. exists y. split; trivial. rewrite filter_spec in *. des.
+    assert (IN : childnodes (unions x1) c \in unions x1) by now eapply member_intro.
+    rewrite -> x_EQ in IN at 2. destruct IN as [c' EQ]. exists c'. rewrite <- EQ. rewrite <- x_EQ. done.
+  - des. exists y. split; trivial. rewrite filter_spec in *. des.
+    assert (IN : childnodes (unions x2) c \in unions x2) by now eapply member_intro.
+    rewrite <- x_EQ in IN at 2. destruct IN as [c' EQ]. exists c'. rewrite <- EQ. rewrite -> x_EQ. done.
+Qed.
+
+Definition snd (t : Tree) : Tree :=
+  unions (filter (fun y => pair (fst t) y == t) (unions t)).
+
+#[global]
+Instance snd_eqPropCompatible1
+  : eqPropCompatible1 snd.
+Proof.
+  ii. unfold snd. eapply eqTree_intro; ii; rewrite unions_spec in *.
+  - des. exists y. split; trivial. rewrite filter_spec in *. des.
+    assert (IN : childnodes (unions x1) c \in unions x1) by now eapply member_intro.
+    rewrite -> x_EQ in IN at 2. destruct IN as [c' EQ]. exists c'. rewrite <- EQ. rewrite <- x_EQ. done.
+  - des. exists y. split; trivial. rewrite filter_spec in *. des.
+    assert (IN : childnodes (unions x2) c \in unions x2) by now eapply member_intro.
+    rewrite <- x_EQ in IN at 2. destruct IN as [c' EQ]. exists c'. rewrite <- EQ. rewrite -> x_EQ. done.
+Qed.
+
+Theorem destruct_pair (t : Tree)
+  (EQ : exists x, exists y, t == pair x y)
+  : t == pair (fst t) (snd t).
+Proof.
+  destruct EQ as (x & y & EQ). rewrite EQ at 1.
+  assert (claim : unions t == upair x y).
+  { eapply eqTree_intro; intros z H_IN.
+    - rewrite EQ in H_IN. rewrite unions_spec in H_IN. destruct H_IN as (w & H_in & H_IN).
+      unfold pair in H_IN. rewrite upair_spec in H_IN. destruct H_IN as [H_EQ | H_EQ]; rewrite H_EQ in H_in; clear w H_EQ.
+      + rewrite upair_spec. left. rewrite <- singlton_spec. exact H_in.
+      + exact H_in.
+    - rewrite upair_spec in H_IN. rewrite EQ. clear t EQ. destruct H_IN as [EQ | EQ].
+      + rewrite unions_spec. exists (singlton x). split.
+        * rewrite singlton_spec. exact EQ.
+        * unfold pair. rewrite upair_spec. now left.
+      + rewrite unions_spec. exists (upair x y). split.
+        * rewrite upair_spec. now right.
+        * unfold pair. rewrite upair_spec. now right.
+  }
+  assert (FST_EQ : x == fst t).
+  { unfold fst. eapply eqTree_intro; intros z H_in.
+    - rewrite unions_spec. exists x. split; trivial. rewrite filter_good.
+      + split.
+        * rewrite claim. rewrite upair_spec. now left.
+        * rewrite EQ. unfold pair. rewrite upair_spec. now left.
+      + intros a H_in' b EQ'. rewrite EQ' in H_in'. exact H_in'.
+    - rewrite unions_spec in H_in. destruct H_in as (w & H_in & H_IN). rewrite filter_good in H_IN.
+      + destruct H_IN as [H_IN1 H_IN2]. rewrite claim in H_IN1.
+        rewrite upair_spec in H_IN1. destruct H_IN1 as [EQ' | EQ']; rewrite EQ' in H_in, H_IN2; clear w EQ'.
+        * exact H_in.
+        * rewrite EQ in H_IN2. unfold pair in H_IN2. rewrite upair_spec in H_IN2. destruct H_IN2 as [EQ' | EQ'].
+          { apply singlton_inj in EQ'. rewrite <- EQ'. exact H_in. }
+          { apply singleton_eq_upair_implies in EQ'. destruct EQ' as [EQ1 EQ2]. rewrite EQ2. exact H_in. }
+      + intros a H_in' b EQ'. rewrite <- EQ'. exact H_in'.
+  }
+  assert (SND_EQ : y == snd t).
+  { unfold snd. eapply eqTree_intro; intros z H_in.
+    - rewrite unions_spec. exists y. split; trivial. rewrite filter_good.
+      + split.
+        * rewrite claim. rewrite upair_spec. now right.
+        * rewrite <- FST_EQ. now rewrite EQ.
+      + intros a H_EQ b EQ'. rewrite <- EQ'. exact H_EQ.
+    - rewrite unions_spec in H_in. destruct H_in as (w & H_in & H_IN). rewrite filter_good in H_IN.
+      + rewrite <- FST_EQ in H_IN. destruct H_IN as [H_IN EQ']. rewrite <- EQ' in EQ. apply pair_inv in EQ.
+        destruct EQ as [_ EQ]. rewrite <- EQ. exact H_in.
+      + intros a H_EQ b EQ'. rewrite <- EQ'. exact H_EQ.
+  }
+  now rewrite FST_EQ, SND_EQ.
+Qed.
+
+Corollary fst_pair x y
+  : fst (pair x y) == x.
+Proof.
+  set (t := pair x y).
+  assert (claim : t == pair (fst t) (snd t)).
+  { eapply destruct_pair. now exists x, y. }
+  unfold t in claim at 1. now apply pair_inv in claim.
+Qed.
+
+Corollary snd_pair x y
+  : snd (pair x y) == y.
+Proof.
+  set (t := pair x y).
+  assert (claim : t == pair (fst t) (snd t)).
+  { eapply destruct_pair. now exists x, y. }
+  unfold t in claim at 1. now apply pair_inv in claim.
 Qed.
 
 End SET_CONSTRUCTIONS.
@@ -335,11 +571,224 @@ Theorem AxiomOfChoice_implies_StrongCollection (P : Tree -> Tree -> Prop)
   : forall X, (forall x, x \in X -> exists y, P x y) -> exists Y, (forall x, x \in X -> exists y, y \in Y /\ P x y) /\ (forall y, y \in Y -> exists x, x \in X /\ P x y).
 Proof with eauto with *.
   intros X NONEMPTY. set (base_set := children X).
-  assert (claim1 : exists f : base_set -> Tree, forall x : base_set, P (childnodes X x) (f x)).
+  assert (claim : exists f : base_set -> Tree, forall x : base_set, P (childnodes X x) (f x)).
   { eapply AC with (P := fun x : base_set => fun y : Tree => P (childnodes X x) y)... }
-  destruct claim1 as [f claim1]. exists (mkNode base_set (fun x => f x)). split.
+  destruct claim as [f claim]. exists (mkNode base_set (fun x => f x)). split.
   - intros x [c EQ]. exists (f c). split... eapply COMPAT1...
   - intros x [c EQ]. exists (childnodes X c). split... eapply COMPAT2...
 Qed.
 
 End STRONG_COLLECTION.
+
+Fixpoint rLe (lhs : Tree) (rhs : Tree) : Prop :=
+  match lhs, rhs with
+  | mkNode cs1 ts1, mkNode cs2 ts2 => forall c1, exists c2, ts1 c1 ≦ᵣ ts2 c2
+  end
+where " lhs ≦ᵣ rhs " := (rLe lhs rhs) : type_scope.
+
+Lemma rLe_refl x
+  : x ≦ᵣ x.
+Proof.
+  induction x as [cx tsx IH]; simpl; eauto with *.
+Qed.
+
+Lemma rLe_trans x y z
+  (LE1 : x ≦ᵣ y)
+  (LE2 : y ≦ᵣ z)
+  : x ≦ᵣ z.
+Proof.
+  revert x y z LE1 LE2.
+  induction x as [nx tsnx IH], y as [ny tsny], z as [nz tsnz]; simpl. intros x2y y2z c.
+  pose proof (x2y c) as [c' LE']. pose proof (y2z c') as [c'' LE'']. eauto with *.
+Qed.
+
+#[global]
+Instance rLe_PreOrder : PreOrder rLe :=
+  { PreOrder_Reflexive := rLe_refl
+  ; PreOrder_Transitive := rLe_trans
+  }.
+
+Definition rEq_asSetoid : isSetoid Tree :=
+  mkSetoidFromPreOrder rLe_PreOrder.
+
+Definition rEq (lhs : Tree) (rhs : Tree) : Prop :=
+  rEq_asSetoid.(eqProp) lhs rhs.
+
+Definition rLt (lhs : Tree) (rhs : Tree) : Prop :=
+  exists witness : children rhs, lhs ≦ᵣ childnodes rhs witness.
+
+Infix "=ᵣ" := rEq (at level 70, no associativity) : type_scope.
+
+Infix "<ᵣ" := rLt (at level 70, no associativity) : type_scope.
+
+#[global] Hint Unfold rEq rLt : aczel_hints.
+
+#[global]
+Instance rEq_Equivalence : Equivalence rEq :=
+  rEq_asSetoid.(eqProp_Equivalence).
+
+#[global]
+Instance rLe_PartialOrder : PartialOrder rEq rLe :=
+  mkSetoidFromPreOrder_derivesPartialOrder rLe_PreOrder.
+
+Lemma rLe_eqTree_rLe x y z
+  (H_rLe : x ≦ᵣ y)
+  (EQ : y == z)
+  : x ≦ᵣ z.
+Proof.
+  revert y z H_rLe EQ. induction x as [csx tsx IH].
+  intros [csy tsy] [csz tsz] H_rLe [y2z z2y] cx. simpl in *.
+  pose proof (H_rLe cx) as [cy ?]. pose proof (y2z cy) as [cz ?]. eauto with *.
+Qed.
+
+Lemma eqTree_rLe_rLe x y z
+  (EQ : x == y)
+  (H_rLe : y ≦ᵣ z)
+  : x ≦ᵣ z.
+Proof.
+  revert y z H_rLe EQ. induction x as [csx tsx IH].
+  intros [csy tsy] [csz tsz] H_rLe [x2y y2x] cx. simpl in *.
+  pose proof (x2y cx) as [cy ?]. pose proof (H_rLe cy) as [cz ?]. eauto with *.
+Qed.
+
+#[global] Hint Resolve rLe_eqTree_rLe eqTree_rLe_rLe : aczel_hints.
+
+#[global]
+Add Parametric Morphism
+  : rLe with signature (eqProp ==> eqProp ==> iff)
+  as rLe_compatWith_eqProp.
+Proof.
+  intros x1 x2 x_EQ y1 y2 y_EQ. split; i.
+  - eapply rLe_eqTree_rLe; eauto. eapply eqTree_rLe_rLe; eauto. done.
+  - eapply rLe_eqTree_rLe; eauto. eapply eqTree_rLe_rLe; eauto. done.
+Qed.
+
+#[global]
+Add Parametric Morphism
+  : rEq with signature (eqProp ==> eqProp ==> iff)
+  as rEq_compatWith_eqProp.
+Proof.
+  intros x1 x2 x_EQ y1 y2 y_EQ. split; intros H_rEq.
+  - do 4 red. do 4 red in H_rEq. rewrite -> x_EQ, -> y_EQ in H_rEq. done.
+  - do 4 red. do 4 red in H_rEq. rewrite <- x_EQ, <- y_EQ in H_rEq. done.
+Qed.
+
+#[global]
+Add Parametric Morphism
+  : rLt with signature (eqProp ==> eqProp ==> iff)
+  as rLt_compatWith_eqProp.
+Proof.
+  intros x1 x2 x_EQ y1 y2 y_EQ. split; intros [c H_rLe].
+  - pose proof (member_intro (children y1) (childnodes y1) c) as IN.
+    rewrite Tree_eta in IN. rewrite -> y_EQ in IN at 2. destruct IN as [c' EQ'].
+    exists c'. rewrite <- EQ'. rewrite <- x_EQ. exact H_rLe.
+  - pose proof (member_intro (children y2) (childnodes y2) c) as IN.
+    rewrite Tree_eta in IN. rewrite <- y_EQ in IN at 2. destruct IN as [c' EQ'].
+    exists c'. rewrite <- EQ'. rewrite -> x_EQ. exact H_rLe.
+Qed.
+
+Lemma rLt_implies_rLe lhs rhs
+  (H_rLt : lhs <ᵣ rhs)
+  : lhs ≦ᵣ rhs.
+Proof.
+  rename lhs into x, rhs into y.
+  destruct H_rLt as [cy H_rLe].
+  rewrite -> H_rLe. clear x H_rLe.
+  induction y as [csy tsy IH]. simpl in *.
+  specialize IH with (c := cy).
+  destruct (tsy cy) as [csz tsz] eqn: cy_EQ_z.
+  intros cz. specialize IH with (cy := cz).
+  rewrite <- cy_EQ_z in IH. eauto with *.
+Qed.
+
+Lemma member_implies_rLt x y
+  (IN : x \in y)
+  : x <ᵣ y.
+Proof.
+  destruct IN as [c EQ]. exists c. eauto with *.
+Qed.
+
+Lemma rLe_rLt_rLt x y z
+  (x_rLe_y : x ≦ᵣ y)
+  (y_rLt_z : y <ᵣ z)
+  : x <ᵣ z.
+Proof.
+  destruct y_rLt_z as [c rLe]. exists c. transitivity y; eauto with *.
+Qed.
+
+Lemma rLt_rLe_rLt x y z
+  (x_rLt_y : x <ᵣ y)
+  (y_rLe_z : y ≦ᵣ z)
+  : x <ᵣ z.
+Proof.
+  destruct y as [csy tsy]. destruct x_rLt_y as [cy x_rLe_cy]. destruct z as [csz tsz].
+  simpl in *. unnw. pose proof (y_rLe_z cy) as [cz cy_rLe_cz]. exists cz. transitivity (tsy cy); eauto with *.
+Qed.
+
+#[local] Hint Resolve rLe_rLt_rLt rLt_rLe_rLt : core.
+
+#[global]
+Add Parametric Morphism
+  : rLt with signature (eqProp ==> eqProp ==> iff) as rLt_compatWith_eq.
+Proof.
+  intros x1 y1 EQ1 x2 y2 EQ2. split; intros [w H_rLe].
+  - eapply rLt_rLe_rLt with (y := x2).
+    + eexists. rewrite <- EQ1. exact H_rLe.
+    + now rewrite -> EQ2.
+  - eapply rLt_rLe_rLt with (y := y2).
+    + eexists. rewrite -> EQ1. exact H_rLe.
+    + now rewrite <- EQ2.
+Qed.
+
+Theorem rLt_wf
+  : well_founded rLt.
+Proof.
+  intros rhs. remember rhs as lhs eqn: lhs_EQ_rhs.
+  assert (lhs_rLe_rhs : lhs ≦ᵣ rhs) by now rewrite lhs_EQ_rhs.
+  clear lhs_EQ_rhs. rename lhs into x, rhs into y, lhs_rLe_rhs into x_rLe_y.
+  revert y x x_rLe_y. induction y as [csy tsy IH].
+  intros [csx tsx] x_rLe_y. simpl in x_rLe_y. unnw.
+  econstructor. intros z [c z_rLe_cx]. simpl in *.
+  pose proof (x_rLe_y c) as [c' H_rLe]. eapply IH; transitivity (tsx c); eauto with *.
+Qed.
+
+Fixpoint fromAcc {A : Type@{Set_u}} {R : A -> A -> Prop} (x : A) (ACC : Acc R x) {struct ACC} : Tree :=
+  match ACC with
+  | Acc_intro _ ACC_INV => mkNode { y : A | R y x } (fun c => @fromAcc A R (proj1_sig c) (ACC_INV (proj1_sig c) (proj2_sig c)))
+  end.
+
+Lemma fromAcc_unfold {A : Type@{Set_u}} {R : A -> A -> Prop} x ACC
+  : forall z, z \in @fromAcc A R x ACC <-> exists c : { y : A | R y x }, z == fromAcc (proj1_sig c) (Acc_inv ACC (proj2_sig c)).
+Proof.
+  intros z. destruct ACC as [ACC_INV]; simpl in *.
+  split; intros [[c H_R] EQ]; rewrite eqTree_unfold in *; now exists (@exist _ _ c H_R).
+Qed.
+
+Fixpoint fromAcc_pirrel (A : Type@{Set_u}) (R : A -> A -> Prop) (x : A) (ACC : Acc R x) (ACC' : Acc R x) {struct ACC}
+  : fromAcc x ACC == fromAcc x ACC'.
+Proof.
+  destruct ACC as [ACC_INV], ACC' as [ACC_INV']. eapply eqTree_intro.
+  - intros z H_in. rewrite fromAcc_unfold in *. destruct H_in as [c EQ].
+    pose proof (fromAcc_pirrel A R (proj1_sig c) (ACC_INV (proj1_sig c) (proj2_sig c)) (ACC_INV' (proj1_sig c) (proj2_sig c))) as claim.
+    exists c. rewrite <- claim. exact EQ.
+  - intros z H_in. rewrite fromAcc_unfold in *. destruct H_in as [c EQ].
+    pose proof (fromAcc_pirrel A R (proj1_sig c) (ACC_INV (proj1_sig c) (proj2_sig c)) (ACC_INV' (proj1_sig c) (proj2_sig c))) as claim.
+    exists c. rewrite -> claim. exact EQ.
+Qed.
+
+Lemma fromAcc_member_fromAcc_intro (A : Type@{Set_u}) (R : A -> A -> Prop) (x : A) (x' : A) (ACC : Acc R x) (ACC' : Acc R x')
+  (R_x_x' : R x x')
+  : fromAcc x ACC \in fromAcc x' ACC'.
+Proof.
+  rewrite fromAcc_unfold. exists (@exist _ _ x R_x_x'). simpl. eapply fromAcc_pirrel.
+Qed.
+
+Corollary fromAcc_rLt_fromAcc_intro (A : Type@{Set_u}) (R : A -> A -> Prop) (x : A) (x' : A) (ACC : Acc R x) (ACC' : Acc R x')
+  (R_x_x' : R x x')
+  : fromAcc x ACC <ᵣ fromAcc x' ACC'.
+Proof.
+  eapply member_implies_rLt. eapply fromAcc_member_fromAcc_intro. exact R_x_x'.
+Qed.
+
+Definition fromWf {A : Type@{Set_u}} {R : A -> A -> Prop} (Wf : well_founded R) : Tree :=
+  indexed_union A (fun i => @fromAcc A R i (Wf i)).
