theories/Prelude/Notations.v
@@ -4,3 +4,8 @@ Reserved Infix "==" (no associativity, at level 70).
 Reserved Infix "=<" (no associativity, at level 70).
 Reserved Infix "\in" (no associativity, at level 70).
 Reserved Infix "\subseteq" (no associativity, at level 70).
+
+Reserved Infix "≦ᵣ" (at level 70, no associativity).
+
+Reserved Infix "=ᵣ" (at level 70, no associativity).
+Reserved Infix "<ᵣ" (at level 70, no associativity).
